src/SchemaWellFormedness.v
@@ -322,3 +322,5 @@ Section WellFormedness.
 
 End WellFormedness.
 
+
+Arguments wfSchema [Name Vals].
